Refactoring TCO into pass 6

06TreeCode/TreeCode.thy
@@ -61,6 +61,7 @@ inductive eval\<^sub>e :: "state\<^sub>e \<Rightarrow> state\<^sub>e \<Rightarro
 | ev\<^sub>e_apply [simp]: "S\<^sub>e (v # Lam\<^sub>e \<Delta>' \<C>' r' # \<V>) ((\<Delta>, Apply\<^sub>e # \<C>, r) # s) \<leadsto>\<^sub>e 
     S\<^sub>e \<V> ((v # \<Delta>', \<C>', r') # (\<Delta>, \<C>, r) # s)"
 | ev\<^sub>e_return [simp]: "S\<^sub>e \<V> ((\<Delta>, [], Return\<^sub>e) # s) \<leadsto>\<^sub>e S\<^sub>e \<V> s"
+| ev\<^sub>e_jump [simp]: "S\<^sub>e (v # Lam\<^sub>e \<Delta>' \<C>' r' # \<V>) ((\<Delta>, [], Jump\<^sub>e) # s) \<leadsto>\<^sub>e S\<^sub>e \<V> ((v # \<Delta>', \<C>', r') # s)"
 
 text \<open>Without typing, our list of safety properties has become quite short: just determinism. We 
 could still type our codeblocks, and thence our state; we would need to give each tree-code 
@@ -86,6 +87,9 @@ next
   thus ?case by (induction rule: eval\<^sub>e.cases) simp_all 
 next
   case ev\<^sub>e_return
+  thus ?case by (induction rule: eval\<^sub>e.cases) simp_all 
+next
+  case ev\<^sub>e_jump
   thus ?case by (induction rule: eval\<^sub>e.cases) simp_all 
 qed
 
