08ByteCode/CodeFlattening.thy
@@ -1,68 +1,68 @@
 theory CodeFlattening
-  imports ByteCode "../07TailCall/TailCall"
+  imports ByteCode "../06TreeCode/TreeCode"
 begin
 
-primrec flatten_return :: "tco_return \<Rightarrow> byte_code" where
-  "flatten_return TCOReturn = BReturn"
-| "flatten_return TCOJump = BJump"
+primrec flatten_return :: "return\<^sub>e \<Rightarrow> byte_code" where
+  "flatten_return Return\<^sub>e = BReturn"
+| "flatten_return Jump\<^sub>e = BJump"
 
-fun flatten_code' :: "nat \<Rightarrow> tco_code list \<Rightarrow> tco_return \<Rightarrow> byte_code list" where
+fun flatten_code' :: "nat \<Rightarrow> code\<^sub>e list \<Rightarrow> return\<^sub>e \<Rightarrow> byte_code list" where
   "flatten_code' lib [] r = [flatten_return r]"
-| "flatten_code' lib (TCOLookup x # cd) r = flatten_code' lib cd r @ [BLookup x]"
-| "flatten_code' lib (TCOPushCon k # cd) r = flatten_code' lib cd r @ [BPushCon k]"
-| "flatten_code' lib (TCOPushLam cd' r' # cd) r = (
+| "flatten_code' lib (Lookup\<^sub>e x # cd) r = flatten_code' lib cd r @ [BLookup x]"
+| "flatten_code' lib (PushCon\<^sub>e k # cd) r = flatten_code' lib cd r @ [BPushCon k]"
+| "flatten_code' lib (PushLam\<^sub>e cd' r' # cd) r = (
     let clo = flatten_code' lib cd' r'
     in clo @ flatten_code' (lib + length clo) cd r @ [BPushLam (lib + length clo)])"
-| "flatten_code' lib (TCOApply # cd) r = flatten_code' lib cd r @ [BApply]"
+| "flatten_code' lib (Apply\<^sub>e # cd) r = flatten_code' lib cd r @ [BApply]"
 
-primrec flatten_code :: "tco_code list \<times> tco_return \<Rightarrow> byte_code list" where
+primrec flatten_code :: "code\<^sub>e list \<times> return\<^sub>e \<Rightarrow> byte_code list" where
   "flatten_code (cd, r) = flatten_code' 0 cd r"
 
-primrec unflatten_return :: "byte_code list \<Rightarrow> nat \<Rightarrow> tco_return" where
+primrec unflatten_return :: "byte_code list \<Rightarrow> nat \<Rightarrow> return\<^sub>e" where
   "unflatten_return cd 0 = undefined"
 | "unflatten_return cd (Suc pc) = (case lookup cd pc of
-      Some BReturn \<Rightarrow> TCOReturn
-    | Some BJump \<Rightarrow> TCOJump
+      Some BReturn \<Rightarrow> Return\<^sub>e
+    | Some BJump \<Rightarrow> Jump\<^sub>e
     | Some op \<Rightarrow> unflatten_return cd pc
     | None \<Rightarrow> undefined)"
 
-fun unflatten_code :: "byte_code list \<Rightarrow> nat \<Rightarrow> tco_code list" where
+fun unflatten_code :: "byte_code list \<Rightarrow> nat \<Rightarrow> code\<^sub>e list" where
   "unflatten_code cd 0 = []"
 | "unflatten_code cd (Suc pc) = (case lookup cd pc of
-      Some (BLookup x) \<Rightarrow> TCOLookup x # unflatten_code cd pc
-    | Some (BPushCon k) \<Rightarrow>  TCOPushCon k # unflatten_code cd pc
+      Some (BLookup x) \<Rightarrow> Lookup\<^sub>e x # unflatten_code cd pc
+    | Some (BPushCon k) \<Rightarrow>  PushCon\<^sub>e k # unflatten_code cd pc
     | Some (BPushLam pc') \<Rightarrow> (
         if pc' \<le> pc 
-        then TCOPushLam (unflatten_code cd pc') (unflatten_return cd pc') # unflatten_code cd pc 
+        then PushLam\<^sub>e (unflatten_code cd pc') (unflatten_return cd pc') # unflatten_code cd pc 
         else undefined) 
-    | Some BApply \<Rightarrow> TCOApply # unflatten_code cd pc
+    | Some BApply \<Rightarrow> Apply\<^sub>e # unflatten_code cd pc
     | Some BReturn \<Rightarrow> []
     | Some BJump \<Rightarrow> []
     | None \<Rightarrow> undefined)"
 
-primrec unflatten_closure :: "byte_code list \<Rightarrow> bclosure \<Rightarrow> tco_closure" where
-  "unflatten_closure cd (BConst k) = TCOConst k"
+primrec unflatten_closure :: "byte_code list \<Rightarrow> bclosure \<Rightarrow> closure\<^sub>e" where
+  "unflatten_closure cd (BConst k) = Const\<^sub>e k"
 | "unflatten_closure cd (BLam vs pc) = 
-    TCOLam (map (unflatten_closure cd) vs) (unflatten_code cd pc) (unflatten_return cd pc)"
+    Lam\<^sub>e (map (unflatten_closure cd) vs) (unflatten_code cd pc) (unflatten_return cd pc)"
 
-abbreviation ufcs :: "byte_code list \<Rightarrow> bclosure list \<Rightarrow> tco_closure list" where
+abbreviation ufcs :: "byte_code list \<Rightarrow> bclosure list \<Rightarrow> closure\<^sub>e list" where
   "ufcs cd vs \<equiv> map (unflatten_closure cd) vs"
 
-primrec ufsf :: "byte_code list \<Rightarrow> (bclosure list \<times> nat) \<Rightarrow> tco_stack_frame" where
+primrec ufsf :: "byte_code list \<Rightarrow> (bclosure list \<times> nat) \<Rightarrow> frame\<^sub>e" where
   "ufsf cd (vs, pc) = (ufcs cd vs, unflatten_code cd pc, unflatten_return cd pc)"
 
-abbreviation ufsfs :: "byte_code list \<Rightarrow> (bclosure list \<times> nat) list \<Rightarrow> tco_stack_frame list" where
+abbreviation ufsfs :: "byte_code list \<Rightarrow> (bclosure list \<times> nat) list \<Rightarrow> frame\<^sub>e list" where
   "ufsfs cd pcs \<equiv> map (ufsf cd) pcs"
 
-primrec unflatten_state :: "byte_code list \<Rightarrow> byte_code_state \<Rightarrow> tco_code_state" where
-  "unflatten_state cd (BS vs sfs) = TCOS (ufcs cd vs) (ufsfs cd sfs)"
+primrec unflatten_state :: "byte_code list \<Rightarrow> byte_code_state \<Rightarrow> state\<^sub>e" where
+  "unflatten_state cd (BS vs sfs) = S\<^sub>e (ufcs cd vs) (ufsfs cd sfs)"
 
-primrec code_size :: "tco_code \<Rightarrow> nat"
-    and code_list_size :: "tco_code list \<Rightarrow> nat" where
-  "code_size (TCOLookup x) = 1"
-| "code_size (TCOPushCon k) = 1"
-| "code_size (TCOPushLam cd r) = Suc (code_list_size cd)"
-| "code_size TCOApply = 1"
+primrec code_size :: "code\<^sub>e \<Rightarrow> nat"
+    and code_list_size :: "code\<^sub>e list \<Rightarrow> nat" where
+  "code_size (Lookup\<^sub>e x) = 1"
+| "code_size (PushCon\<^sub>e k) = 1"
+| "code_size (PushLam\<^sub>e cd r) = Suc (code_list_size cd)"
+| "code_size Apply\<^sub>e = 1"
 | "code_list_size [] = 1"
 | "code_list_size (c # cd) = code_size c + code_list_size cd"
 
@@ -248,181 +248,181 @@ lemma [simp]: "lookup cd pc = Some (BPushLam pc') \<Longrightarrow> orderly cd 0
   using orderly_lam by fastforce
 
 theorem correctb [simp]: "cd \<tturnstile> \<Sigma>\<^sub>b \<leadsto>\<^sub>b \<Sigma>\<^sub>b' \<Longrightarrow> orderly_state cd \<Sigma>\<^sub>b \<Longrightarrow> 
-  iter (\<leadsto>\<^sub>e\<^sub>c\<^sub>o) (unflatten_state cd \<Sigma>\<^sub>b) (unflatten_state cd \<Sigma>\<^sub>b')"
+  iter (\<leadsto>\<^sub>e) (unflatten_state cd \<Sigma>\<^sub>b) (unflatten_state cd \<Sigma>\<^sub>b')"
 proof (induction \<Sigma>\<^sub>b \<Sigma>\<^sub>b' rule: evalb.induct)
   case (evb_lookup cd pc x env v vs sfs)
-  hence "TCOS (ufcs cd vs) 
-    ((ufcs cd env, unflatten_code cd (Suc pc), unflatten_return cd (Suc pc)) # ufsfs cd sfs) \<leadsto>\<^sub>e\<^sub>c\<^sub>o
-      TCOS (unflatten_closure cd v # ufcs cd vs)
+  hence "S\<^sub>e (ufcs cd vs) 
+    ((ufcs cd env, unflatten_code cd (Suc pc), unflatten_return cd (Suc pc)) # ufsfs cd sfs) \<leadsto>\<^sub>e
+      S\<^sub>e (unflatten_closure cd v # ufcs cd vs)
         ((ufcs cd env, unflatten_code cd pc, unflatten_return cd pc) # ufsfs cd sfs)" by simp
   thus ?case by simp
 next
   case (evb_pushcon cd pc k vs env sfs)
-  hence "TCOS (ufcs cd vs) 
-    ((ufcs cd env, unflatten_code cd (Suc pc), unflatten_return cd (Suc pc)) # ufsfs cd sfs) \<leadsto>\<^sub>e\<^sub>c\<^sub>o
-      TCOS (TCOConst k # ufcs cd vs) 
+  hence "S\<^sub>e (ufcs cd vs) 
+    ((ufcs cd env, unflatten_code cd (Suc pc), unflatten_return cd (Suc pc)) # ufsfs cd sfs) \<leadsto>\<^sub>e
+      S\<^sub>e (Const\<^sub>e k # ufcs cd vs) 
         ((ufcs cd env, unflatten_code cd pc, unflatten_return cd pc) # ufsfs cd sfs)" by simp
   thus ?case by simp
 next
   case (evb_pushlam cd pc pc' vs env sfs)
   moreover hence X: "pc' \<le> pc" by auto
-  moreover have "iter (\<leadsto>\<^sub>e\<^sub>c\<^sub>o) (TCOS (ufcs cd vs) ((ufcs cd env, 
-    TCOPushLam (unflatten_code cd pc') (unflatten_return cd pc') # 
+  moreover have "iter (\<leadsto>\<^sub>e) (S\<^sub>e (ufcs cd vs) ((ufcs cd env, 
+    PushLam\<^sub>e (unflatten_code cd pc') (unflatten_return cd pc') # 
       unflatten_code cd pc, unflatten_return cd pc) # ufsfs cd sfs))
-        (TCOS (TCOLam (ufcs cd env) (unflatten_code cd pc') (unflatten_return cd pc') # ufcs cd vs) 
+        (S\<^sub>e (Lam\<^sub>e (ufcs cd env) (unflatten_code cd pc') (unflatten_return cd pc') # ufcs cd vs) 
           ((ufcs cd env, unflatten_code cd pc, unflatten_return cd pc) # ufsfs cd sfs))" 
-    by (metis evtco_pushlam iter_one)
+    by (metis ev\<^sub>e_pushlam iter_one)
   ultimately show ?case by simp
 next
   case (evb_apply cd pc v env' pc' vs env sfs)
-  hence "TCOS (unflatten_closure cd v # TCOLam (ufcs cd env') (unflatten_code cd pc') 
+  hence "S\<^sub>e (unflatten_closure cd v # Lam\<^sub>e (ufcs cd env') (unflatten_code cd pc') 
     (unflatten_return cd pc') # ufcs cd vs) 
-      ((ufcs cd env, unflatten_code cd (Suc pc), unflatten_return cd (Suc pc)) # ufsfs cd sfs) \<leadsto>\<^sub>e\<^sub>c\<^sub>o
-        TCOS (ufcs cd vs) ((unflatten_closure cd v # ufcs cd env', unflatten_code cd pc', 
+      ((ufcs cd env, unflatten_code cd (Suc pc), unflatten_return cd (Suc pc)) # ufsfs cd sfs) \<leadsto>\<^sub>e
+        S\<^sub>e (ufcs cd vs) ((unflatten_closure cd v # ufcs cd env', unflatten_code cd pc', 
           unflatten_return cd pc') # (ufcs cd env, unflatten_code cd pc, unflatten_return cd pc) # 
             ufsfs cd sfs)" by simp
   thus ?case by simp
 next
   case (evb_return cd pc vs env sfs)
-  moreover have "iter (\<leadsto>\<^sub>e\<^sub>c\<^sub>o) (TCOS (ufcs cd vs) ((ufcs cd env, [], TCOReturn) # ufsfs cd sfs))
-    (TCOS (ufcs cd vs) (ufsfs cd sfs))" by (metis evtco_return iter_one)
+  moreover have "iter (\<leadsto>\<^sub>e) (S\<^sub>e (ufcs cd vs) ((ufcs cd env, [], Return\<^sub>e) # ufsfs cd sfs))
+    (S\<^sub>e (ufcs cd vs) (ufsfs cd sfs))" by (metis ev\<^sub>e_return iter_one)
   ultimately show ?case by simp
 next
   case (evb_jump cd pc v env' pc' vs env sfs)
-  have "TCOS (unflatten_closure cd v # TCOLam (ufcs cd env') (unflatten_code cd pc') 
+  have "S\<^sub>e (unflatten_closure cd v # Lam\<^sub>e (ufcs cd env') (unflatten_code cd pc') 
     (unflatten_return cd pc') # ufcs cd vs) ((ufcs cd env, [], 
-      TCOJump) # ufsfs cd sfs) \<leadsto>\<^sub>e\<^sub>c\<^sub>o TCOS (ufcs cd vs)
+      Jump\<^sub>e) # ufsfs cd sfs) \<leadsto>\<^sub>e S\<^sub>e (ufcs cd vs)
         ((unflatten_closure cd v # ufcs cd env', unflatten_code cd pc', unflatten_return cd pc') # 
-          ufsfs cd sfs)" by (metis evtco_jump)
-  with evb_jump have "TCOS (unflatten_closure cd v # 
-    TCOLam (ufcs cd env') (unflatten_code cd pc') (unflatten_return cd pc') # ufcs cd vs)
-      ((ufcs cd env, unflatten_code cd (Suc pc), unflatten_return cd (Suc pc)) # ufsfs cd sfs) \<leadsto>\<^sub>e\<^sub>c\<^sub>o
-        TCOS (ufcs cd vs) ((unflatten_closure cd v # ufcs cd env', unflatten_code cd pc', 
+          ufsfs cd sfs)" by (metis ev\<^sub>e_jump)
+  with evb_jump have "S\<^sub>e (unflatten_closure cd v # 
+    Lam\<^sub>e (ufcs cd env') (unflatten_code cd pc') (unflatten_return cd pc') # ufcs cd vs)
+      ((ufcs cd env, unflatten_code cd (Suc pc), unflatten_return cd (Suc pc)) # ufsfs cd sfs) \<leadsto>\<^sub>e
+        S\<^sub>e (ufcs cd vs) ((unflatten_closure cd v # ufcs cd env', unflatten_code cd pc', 
           unflatten_return cd pc') # ufsfs cd sfs)" by simp
-  hence "iter (\<leadsto>\<^sub>e\<^sub>c\<^sub>o) (TCOS (unflatten_closure cd v # 
-    TCOLam (ufcs cd env') (unflatten_code cd pc') (unflatten_return cd pc') # ufcs cd vs)
+  hence "iter (\<leadsto>\<^sub>e) (S\<^sub>e (unflatten_closure cd v # 
+    Lam\<^sub>e (ufcs cd env') (unflatten_code cd pc') (unflatten_return cd pc') # ufcs cd vs)
       ((ufcs cd env, unflatten_code cd (Suc pc), unflatten_return cd (Suc pc)) # ufsfs cd sfs))
-        (TCOS (ufcs cd vs) ((unflatten_closure cd v # ufcs cd env', unflatten_code cd pc', 
+        (S\<^sub>e (ufcs cd vs) ((unflatten_closure cd v # ufcs cd env', unflatten_code cd pc', 
           unflatten_return cd pc') # ufsfs cd sfs))" by (metis iter_one)
   thus ?case by simp
 qed
 
-lemma [simp]: "TCOLam envt cdt rt = unflatten_closure cdb vb \<Longrightarrow> 
+lemma [simp]: "Lam\<^sub>e envt cdt rt = unflatten_closure cdb vb \<Longrightarrow> 
   \<exists>envb pc. vb = BLam envb pc \<and> envt = ufcs cdb envb \<and> cdt = unflatten_code cdb pc \<and>
     rt = unflatten_return cdb pc"
   by (induction vb) simp_all
 
-lemma unfl_state [dest]: "TCOS vs sfs = unflatten_state cd \<Sigma>\<^sub>b \<Longrightarrow> \<exists>vsb sfsb. 
+lemma unfl_state [dest]: "S\<^sub>e vs sfs = unflatten_state cd \<Sigma>\<^sub>b \<Longrightarrow> \<exists>vsb sfsb. 
     \<Sigma>\<^sub>b = BS vsb sfsb \<and> vs = ufcs cd vsb \<and> sfs = ufsfs cd sfsb"
   by (induction \<Sigma>\<^sub>b) simp_all
 
-lemma [dest]: "TCOLookup x # cdt = unflatten_code cdb (Suc pc) \<Longrightarrow> orderly cdb 0 \<Longrightarrow> 
+lemma [dest]: "Lookup\<^sub>e x # cdt = unflatten_code cdb (Suc pc) \<Longrightarrow> orderly cdb 0 \<Longrightarrow> 
     pc < length cdb \<Longrightarrow> lookup cdb pc = Some (BLookup x) \<and> cdt = unflatten_code cdb pc"
   by (simp split: option.splits byte_code.splits)
 
-lemma [dest]: "TCOPushCon k # cdt = unflatten_code cdb (Suc pc) \<Longrightarrow> orderly cdb 0 \<Longrightarrow> 
+lemma [dest]: "PushCon\<^sub>e k # cdt = unflatten_code cdb (Suc pc) \<Longrightarrow> orderly cdb 0 \<Longrightarrow> 
     pc < length cdb \<Longrightarrow> lookup cdb pc = Some (BPushCon k) \<and> cdt = unflatten_code cdb pc"
   by (simp split: option.splits byte_code.splits)
 
-lemma [dest]: "TCOPushLam cdt'' r # cdt = unflatten_code cdb (Suc pc) \<Longrightarrow> 
+lemma [dest]: "PushLam\<^sub>e cdt'' r # cdt = unflatten_code cdb (Suc pc) \<Longrightarrow> 
   orderly cdb 0 \<Longrightarrow> pc < length cdb \<Longrightarrow>  
     \<exists>pc'. lookup cdb pc = Some (BPushLam pc') \<and> cdt = unflatten_code cdb pc \<and> 
       cdt'' = unflatten_code cdb pc' \<and> r = unflatten_return cdb pc'"
   by (simp split: option.splits byte_code.splits)
 
-lemma [dest]: "TCOApply # cdt = unflatten_code cdb (Suc pc) \<Longrightarrow> orderly cdb 0 \<Longrightarrow> 
+lemma [dest]: "Apply\<^sub>e # cdt = unflatten_code cdb (Suc pc) \<Longrightarrow> orderly cdb 0 \<Longrightarrow> 
     pc < length cdb \<Longrightarrow> lookup cdb pc = Some BApply \<and> cdt = unflatten_code cdb pc"
   by (simp split: option.splits byte_code.splits)
 
-lemma [dest]: "[] = unflatten_code cdb (Suc pc) \<Longrightarrow> TCOReturn = unflatten_return cdb (Suc pc) \<Longrightarrow> 
+lemma [dest]: "[] = unflatten_code cdb (Suc pc) \<Longrightarrow> Return\<^sub>e = unflatten_return cdb (Suc pc) \<Longrightarrow> 
     orderly cdb 0 \<Longrightarrow> pc < length cdb \<Longrightarrow> lookup cdb pc = Some BReturn"
   by (simp split: option.splits byte_code.splits)
 
-lemma [dest]: "[] = unflatten_code cdb (Suc pc) \<Longrightarrow> TCOJump = unflatten_return cdb (Suc pc) \<Longrightarrow> 
+lemma [dest]: "[] = unflatten_code cdb (Suc pc) \<Longrightarrow> Jump\<^sub>e = unflatten_return cdb (Suc pc) \<Longrightarrow> 
     orderly cdb 0 \<Longrightarrow> pc < length cdb \<Longrightarrow> lookup cdb pc = Some BJump"
   by (simp split: option.splits byte_code.splits)
 
-lemma uf_to_lookup [dest]: "(envt, TCOLookup x # cdt, r) # sfst = ufsfs cdb sfsb \<Longrightarrow> 
+lemma uf_to_lookup [dest]: "(envt, Lookup\<^sub>e x # cdt, r) # sfst = ufsfs cdb sfsb \<Longrightarrow> 
   orderly cdb 0 \<Longrightarrow> orderly_stack sfsb (length cdb) \<Longrightarrow> \<exists>envb pc sfsb'. 
     sfsb = (envb, Suc pc) # sfsb' \<and> envt = ufcs cdb envb \<and> lookup cdb pc = Some (BLookup x) \<and> 
       cdt = unflatten_code cdb pc \<and> r = unflatten_return cdb pc \<and> sfst = ufsfs cdb sfsb'"
 proof (induction sfsb "length cdb" rule: orderly_stack.induct)
   case (3 envb pc sfsb')
-  hence "TCOLookup x # cdt = unflatten_code cdb (Suc pc) \<and> orderly cdb 0 \<and> pc < length cdb" by simp
+  hence "Lookup\<^sub>e x # cdt = unflatten_code cdb (Suc pc) \<and> orderly cdb 0 \<and> pc < length cdb" by simp
   hence "lookup cdb pc = Some (BLookup x) \<and> cdt = unflatten_code cdb pc" by blast
   with 3 show ?case by simp
 qed simp_all
 
-lemma uf_to_pushcon [dest]: "(envt, TCOPushCon k # cdt, r) # sfst = ufsfs cdb sfsb \<Longrightarrow> 
+lemma uf_to_pushcon [dest]: "(envt, PushCon\<^sub>e k # cdt, r) # sfst = ufsfs cdb sfsb \<Longrightarrow> 
   orderly cdb 0 \<Longrightarrow> orderly_stack sfsb (length cdb) \<Longrightarrow> 
     \<exists>envb pc sfsb'. sfsb = (envb, Suc pc) # sfsb' \<and> envt = ufcs cdb envb \<and> 
       lookup cdb pc = Some (BPushCon k) \<and> cdt = unflatten_code cdb pc \<and> 
         r = unflatten_return cdb pc \<and> sfst = ufsfs cdb sfsb'"
 proof (induction sfsb "length cdb" rule: orderly_stack.induct)
   case (3 envb pc sfsb')
-  hence "TCOPushCon k # cdt = unflatten_code cdb (Suc pc) \<and> orderly cdb 0 \<and> pc < length cdb" by simp
+  hence "PushCon\<^sub>e k # cdt = unflatten_code cdb (Suc pc) \<and> orderly cdb 0 \<and> pc < length cdb" by simp
   hence "lookup cdb pc = Some (BPushCon k) \<and> cdt = unflatten_code cdb pc" by blast
   with 3 show ?case by simp
 qed simp_all
 
-lemma uf_to_pushlam [dest]: "(envt, TCOPushLam cdt' r' # cdt, r) # sfst = ufsfs cdb sfsb \<Longrightarrow> 
+lemma uf_to_pushlam [dest]: "(envt, PushLam\<^sub>e cdt' r' # cdt, r) # sfst = ufsfs cdb sfsb \<Longrightarrow> 
   orderly cdb 0 \<Longrightarrow> orderly_stack sfsb (length cdb) \<Longrightarrow> \<exists>envb pc sfsb' pc'. 
     sfsb = (envb, Suc pc) # sfsb' \<and> envt = ufcs cdb envb \<and> lookup cdb pc = Some (BPushLam pc') \<and> 
       cdt = unflatten_code cdb pc \<and> r = unflatten_return cdb pc \<and> cdt' = unflatten_code cdb pc' \<and> 
         r' = unflatten_return cdb pc' \<and> sfst = ufsfs cdb sfsb'"
 proof (induction sfsb "length cdb" rule: orderly_stack.induct)
   case (3 envb pc sfsb')
-  hence "TCOPushLam cdt' r' # cdt = unflatten_code cdb (Suc pc) \<and> orderly cdb 0 \<and> pc < length cdb" 
+  hence "PushLam\<^sub>e cdt' r' # cdt = unflatten_code cdb (Suc pc) \<and> orderly cdb 0 \<and> pc < length cdb" 
     by simp
   then obtain pc' where "lookup cdb pc = Some (BPushLam pc') \<and> cdt = unflatten_code cdb pc \<and> 
     cdt' = unflatten_code cdb pc' \<and> r' = unflatten_return cdb pc'" by blast
   with 3 show ?case by simp
 qed simp_all
 
-lemma uf_to_apply [dest]: "(envt, TCOApply # cdt, r) # sfst = ufsfs cdb sfsb \<Longrightarrow> orderly cdb 0 \<Longrightarrow> 
+lemma uf_to_apply [dest]: "(envt, Apply\<^sub>e # cdt, r) # sfst = ufsfs cdb sfsb \<Longrightarrow> orderly cdb 0 \<Longrightarrow> 
   orderly_stack sfsb (length cdb) \<Longrightarrow> \<exists>envb pc sfsb'. sfsb = (envb, Suc pc) # sfsb' \<and> 
     envt = ufcs cdb envb \<and> lookup cdb pc = Some BApply \<and> cdt = unflatten_code cdb pc \<and> 
       r = unflatten_return cdb pc \<and> sfst = ufsfs cdb sfsb'"
 proof (induction sfsb "length cdb" rule: orderly_stack.induct)
   case (3 envb pc sfsb')
-  hence "TCOApply # cdt = unflatten_code cdb (Suc pc) \<and> orderly cdb 0 \<and> pc < length cdb" by simp
+  hence "Apply\<^sub>e # cdt = unflatten_code cdb (Suc pc) \<and> orderly cdb 0 \<and> pc < length cdb" by simp
   hence "lookup cdb pc = Some BApply \<and> cdt = unflatten_code cdb pc" by blast
   with 3 show ?case by simp
 qed simp_all
 
-lemma uf_to_return [dest]: "(envt, [], TCOReturn) # sfst = ufsfs cdb sfsb \<Longrightarrow> orderly cdb 0 \<Longrightarrow> 
+lemma uf_to_return [dest]: "(envt, [], Return\<^sub>e) # sfst = ufsfs cdb sfsb \<Longrightarrow> orderly cdb 0 \<Longrightarrow> 
   orderly_stack sfsb (length cdb) \<Longrightarrow> \<exists>envb pc sfsb'. sfsb = (envb, Suc pc) # sfsb' \<and> 
     envt = ufcs cdb envb \<and> lookup cdb pc = Some BReturn \<and> sfst = ufsfs cdb sfsb'"
 proof (induction sfsb "length cdb" rule: orderly_stack.induct)
   case (3 envb pc sfsb')
-  hence "[] = unflatten_code cdb (Suc pc) \<and> TCOReturn = unflatten_return cdb (Suc pc) \<and> 
+  hence "[] = unflatten_code cdb (Suc pc) \<and> Return\<^sub>e = unflatten_return cdb (Suc pc) \<and> 
     orderly cdb 0 \<and> pc < length cdb" by simp
   hence "lookup cdb pc = Some BReturn" by blast
   with 3 show ?case by simp
 qed simp_all
 
-lemma uf_to_jump [dest]: "(envt, [], TCOJump) # sfst = ufsfs cdb sfsb \<Longrightarrow> orderly cdb 0 \<Longrightarrow> 
+lemma uf_to_jump [dest]: "(envt, [], Jump\<^sub>e) # sfst = ufsfs cdb sfsb \<Longrightarrow> orderly cdb 0 \<Longrightarrow> 
   orderly_stack sfsb (length cdb) \<Longrightarrow> \<exists>envb pc sfsb'. sfsb = (envb, Suc pc) # sfsb' \<and> 
     envt = ufcs cdb envb \<and> lookup cdb pc = Some BJump \<and> sfst = ufsfs cdb sfsb'"
 proof (induction sfsb "length cdb" rule: orderly_stack.induct)
   case (3 envb pc sfsb')
-  hence "[] = unflatten_code cdb (Suc pc) \<and> TCOJump = unflatten_return cdb (Suc pc) \<and> 
+  hence "[] = unflatten_code cdb (Suc pc) \<and> Jump\<^sub>e = unflatten_return cdb (Suc pc) \<and> 
     orderly cdb 0 \<and> pc < length cdb" by simp
   hence "lookup cdb pc = Some BJump" by blast
   with 3 show ?case by simp
 qed simp_all
 
-theorem completeb [simp]: "unflatten_state cd\<^sub>b \<Sigma>\<^sub>b \<leadsto>\<^sub>e\<^sub>c\<^sub>o \<Sigma>\<^sub>t' \<Longrightarrow> orderly_state cd\<^sub>b \<Sigma>\<^sub>b \<Longrightarrow>
+theorem completeb [simp]: "unflatten_state cd\<^sub>b \<Sigma>\<^sub>b \<leadsto>\<^sub>e \<Sigma>\<^sub>t' \<Longrightarrow> orderly_state cd\<^sub>b \<Sigma>\<^sub>b \<Longrightarrow>
   \<exists>\<Sigma>\<^sub>b'. iter (\<tturnstile> cd\<^sub>b \<leadsto>\<^sub>b) \<Sigma>\<^sub>b \<Sigma>\<^sub>b' \<and> unflatten_state cd\<^sub>b \<Sigma>\<^sub>b' = \<Sigma>\<^sub>t'"
-proof (induction "unflatten_state cd\<^sub>b \<Sigma>\<^sub>b" \<Sigma>\<^sub>t' rule: evaltco.induct)
-  case (evtco_lookup env x v vs cd r sfs)
+proof (induction "unflatten_state cd\<^sub>b \<Sigma>\<^sub>b" \<Sigma>\<^sub>t' rule: eval\<^sub>e.induct)
+  case (ev\<^sub>e_lookup env x v vs cd r sfs)
   then obtain vsb sfsb where B: "\<Sigma>\<^sub>b = BS vsb sfsb \<and> vs = ufcs cd\<^sub>b vsb \<and> 
-    (env, TCOLookup x # cd, r) # sfs = ufsfs cd\<^sub>b sfsb" by fastforce
-  with evtco_lookup have "orderly cd\<^sub>b 0 \<and> orderly_stack sfsb (length cd\<^sub>b)" by simp
+    (env, Lookup\<^sub>e x # cd, r) # sfs = ufsfs cd\<^sub>b sfsb" by fastforce
+  with ev\<^sub>e_lookup have "orderly cd\<^sub>b 0 \<and> orderly_stack sfsb (length cd\<^sub>b)" by simp
   with B obtain envb pc sfsb' where S: "sfsb = (envb, Suc pc) # sfsb' \<and> 
     env = ufcs cd\<^sub>b envb \<and> lookup cd\<^sub>b pc = Some (BLookup x) \<and> cd = unflatten_code cd\<^sub>b pc \<and> 
       r = unflatten_return cd\<^sub>b pc \<and> sfs = ufsfs cd\<^sub>b sfsb'" by (metis uf_to_lookup)
-  with evtco_lookup obtain v' where V: "lookup envb x = Some v' \<and> unflatten_closure cd\<^sub>b v' = v"
+  with ev\<^sub>e_lookup obtain v' where V: "lookup envb x = Some v' \<and> unflatten_closure cd\<^sub>b v' = v"
     by fastforce
   with S have "cd\<^sub>b \<tturnstile> BS vsb ((envb, Suc pc) # sfsb') \<leadsto>\<^sub>b BS (v' # vsb) ((envb, pc) # sfsb')"
     by simp
@@ -430,10 +430,10 @@ proof (induction "unflatten_state cd\<^sub>b \<Sigma>\<^sub>b" \<Sigma>\<^sub>t'
     by simp
   with B S V show ?case by fastforce
 next
-  case (evtco_pushcon vs env k cd r sfs)
+  case (ev\<^sub>e_pushcon vs env k cd r sfs)
   then obtain vsb sfsb where B: "\<Sigma>\<^sub>b = BS vsb sfsb \<and> vs = ufcs cd\<^sub>b vsb \<and> 
-    (env, TCOPushCon k # cd, r) # sfs = ufsfs cd\<^sub>b sfsb" by fastforce
-  with evtco_pushcon have "orderly cd\<^sub>b 0 \<and> orderly_stack sfsb (length cd\<^sub>b)" by simp
+    (env, PushCon\<^sub>e k # cd, r) # sfs = ufsfs cd\<^sub>b sfsb" by fastforce
+  with ev\<^sub>e_pushcon have "orderly cd\<^sub>b 0 \<and> orderly_stack sfsb (length cd\<^sub>b)" by simp
   with B obtain envb pc sfsb' where S: "sfsb = (envb, Suc pc) # sfsb' \<and> 
     env = ufcs cd\<^sub>b envb \<and> lookup cd\<^sub>b pc = Some (BPushCon k) \<and> cd = unflatten_code cd\<^sub>b pc \<and> 
       r = unflatten_return cd\<^sub>b pc \<and> sfs = ufsfs cd\<^sub>b sfsb'" by (metis uf_to_pushcon)
@@ -443,10 +443,10 @@ next
     (BS (BConst k # vsb) ((envb, pc) # sfsb'))" by simp
   with B S show ?case by fastforce
 next
-  case (evtco_pushlam vs env cd' r' cd r sfs)
+  case (ev\<^sub>e_pushlam vs env cd' r' cd r sfs)
   then obtain vsb sfsb where B: "\<Sigma>\<^sub>b = BS vsb sfsb \<and> vs = ufcs cd\<^sub>b vsb \<and> 
-    (env, TCOPushLam cd' r' # cd, r) # sfs = ufsfs cd\<^sub>b sfsb" by fastforce
-  with evtco_pushlam have "orderly cd\<^sub>b 0 \<and> orderly_stack sfsb (length cd\<^sub>b)" by simp
+    (env, PushLam\<^sub>e cd' r' # cd, r) # sfs = ufsfs cd\<^sub>b sfsb" by fastforce
+  with ev\<^sub>e_pushlam have "orderly cd\<^sub>b 0 \<and> orderly_stack sfsb (length cd\<^sub>b)" by simp
   with B obtain envb pc sfsb' pc' where S: "sfsb = (envb, Suc pc) # sfsb' \<and> 
     env = ufcs cd\<^sub>b envb \<and> lookup cd\<^sub>b pc = Some (BPushLam pc') \<and> cd = unflatten_code cd\<^sub>b pc \<and> 
       r = unflatten_return cd\<^sub>b pc \<and> sfs = ufsfs cd\<^sub>b sfsb' \<and> cd' = unflatten_code cd\<^sub>b pc' \<and> 
@@ -457,11 +457,11 @@ next
     (BS (BLam envb pc' # vsb) ((envb, pc) # sfsb'))" by simp
   with B S show ?case by fastforce
 next
-  case (evtco_apply v env' cd' r' vs env cd r sfs)
+  case (ev\<^sub>e_apply v env' cd' r' vs env cd r sfs)
   then obtain vsb sfsb where B: "\<Sigma>\<^sub>b = BS vsb sfsb \<and> 
-    v # TCOLam env' cd' r' # vs = ufcs cd\<^sub>b vsb \<and> (env, TCOApply # cd, r) # sfs = ufsfs cd\<^sub>b sfsb" 
+    v # Lam\<^sub>e env' cd' r' # vs = ufcs cd\<^sub>b vsb \<and> (env, Apply\<^sub>e # cd, r) # sfs = ufsfs cd\<^sub>b sfsb" 
       by fastforce
-  with evtco_apply have "orderly cd\<^sub>b 0 \<and> orderly_stack sfsb (length cd\<^sub>b)" by simp
+  with ev\<^sub>e_apply have "orderly cd\<^sub>b 0 \<and> orderly_stack sfsb (length cd\<^sub>b)" by simp
   with B obtain envb pc sfsb' where S: "sfsb = (envb, Suc pc) # sfsb' \<and> 
     env = ufcs cd\<^sub>b envb \<and> lookup cd\<^sub>b pc = Some BApply \<and> cd = unflatten_code cd\<^sub>b pc \<and> 
       r = unflatten_return cd\<^sub>b pc \<and> sfs = ufsfs cd\<^sub>b sfsb'" by (metis uf_to_apply)
@@ -474,10 +474,10 @@ next
     (BS vsb' ((vb # envb', pc') # (envb, pc) # sfsb'))" by simp
   with B S V show ?case by auto                                              
 next
-  case (evtco_return vs env sfs)
+  case (ev\<^sub>e_return vs env sfs)
   then obtain vsb sfsb where B: "\<Sigma>\<^sub>b = BS vsb sfsb \<and> vs = ufcs cd\<^sub>b vsb \<and> 
-    (env, [], TCOReturn) # sfs = ufsfs cd\<^sub>b sfsb" by fastforce
-  with evtco_return have "orderly cd\<^sub>b 0 \<and> orderly_stack sfsb (length cd\<^sub>b)" by simp
+    (env, [], Return\<^sub>e) # sfs = ufsfs cd\<^sub>b sfsb" by fastforce
+  with ev\<^sub>e_return have "orderly cd\<^sub>b 0 \<and> orderly_stack sfsb (length cd\<^sub>b)" by simp
   with B obtain envb pc sfsb' where S: "sfsb = (envb, Suc pc) # sfsb' \<and> 
     env = ufcs cd\<^sub>b envb \<and> lookup cd\<^sub>b pc = Some BReturn \<and> sfs = ufsfs cd\<^sub>b sfsb'" 
       by (metis uf_to_return)
@@ -485,11 +485,11 @@ next
   hence "iter (\<tturnstile> cd\<^sub>b \<leadsto>\<^sub>b) (BS vsb ((envb, Suc pc) # sfsb')) (BS vsb sfsb')" by simp
   with B S show ?case by fastforce
 next
-  case (evtco_jump v env' cd' r' vs env sfs)
+  case (ev\<^sub>e_jump v env' cd' r' vs env sfs)
   then obtain vsb sfsb where B: "\<Sigma>\<^sub>b = BS vsb sfsb \<and> 
-    v # TCOLam env' cd' r' # vs = ufcs cd\<^sub>b vsb \<and> 
-      (env, [], TCOJump) # sfs = ufsfs cd\<^sub>b sfsb" by fastforce
-  with evtco_jump have "orderly cd\<^sub>b 0 \<and> orderly_stack sfsb (length cd\<^sub>b)" by simp
+    v # Lam\<^sub>e env' cd' r' # vs = ufcs cd\<^sub>b vsb \<and> 
+      (env, [], Jump\<^sub>e) # sfs = ufsfs cd\<^sub>b sfsb" by fastforce
+  with ev\<^sub>e_jump have "orderly cd\<^sub>b 0 \<and> orderly_stack sfsb (length cd\<^sub>b)" by simp
   with B obtain envb pc sfsb' where S: "sfsb = (envb, Suc pc) # sfsb' \<and> 
     env = ufcs cd\<^sub>b envb \<and> lookup cd\<^sub>b pc = Some BJump \<and> sfs = ufsfs cd\<^sub>b sfsb'" 
       by (metis uf_to_jump)
@@ -528,7 +528,7 @@ qed simp_all
 lemma [simp]: "iter (\<tturnstile> cd\<^sub>b \<leadsto>\<^sub>b) \<Sigma>\<^sub>b \<Sigma>\<^sub>b' \<Longrightarrow> orderly_state cd\<^sub>b \<Sigma>\<^sub>b \<Longrightarrow> orderly_state cd\<^sub>b \<Sigma>\<^sub>b'"
   by (induction \<Sigma>\<^sub>b \<Sigma>\<^sub>b' rule: iter.induct) simp_all
 
-lemma [simp]: "iter (\<leadsto>\<^sub>e\<^sub>c\<^sub>o) (unflatten_state cd\<^sub>b \<Sigma>\<^sub>b) \<Sigma>\<^sub>t' \<Longrightarrow> orderly_state cd\<^sub>b \<Sigma>\<^sub>b \<Longrightarrow>
+lemma [simp]: "iter (\<leadsto>\<^sub>e) (unflatten_state cd\<^sub>b \<Sigma>\<^sub>b) \<Sigma>\<^sub>t' \<Longrightarrow> orderly_state cd\<^sub>b \<Sigma>\<^sub>b \<Longrightarrow>
   \<exists>\<Sigma>\<^sub>b'. iter (\<tturnstile> cd\<^sub>b \<leadsto>\<^sub>b) \<Sigma>\<^sub>b \<Sigma>\<^sub>b' \<and> unflatten_state cd\<^sub>b \<Sigma>\<^sub>b' = \<Sigma>\<^sub>t'"
 proof (induction "unflatten_state cd\<^sub>b \<Sigma>\<^sub>b" \<Sigma>\<^sub>t' arbitrary: \<Sigma>\<^sub>b rule: iter.induct)
   case (iter_step \<Sigma>\<^sub>t' \<Sigma>\<^sub>t'')
@@ -540,23 +540,23 @@ proof (induction "unflatten_state cd\<^sub>b \<Sigma>\<^sub>b" \<Sigma>\<^sub>t'
   with S show ?case by (metis iter_append)
 qed force+
 
-lemma unfl_terminal [simp]: "unflatten_state cd \<Sigma> = TCOS [c] [] \<Longrightarrow>
+lemma unfl_terminal [simp]: "unflatten_state cd \<Sigma> = S\<^sub>e [c] [] \<Longrightarrow>
   \<exists>v. \<Sigma> = BS [v] [] \<and> c = unflatten_closure cd v"
 proof -
-  assume "unflatten_state cd \<Sigma> = TCOS [c] []"
+  assume "unflatten_state cd \<Sigma> = S\<^sub>e [c] []"
   then obtain vs sfs where S: "\<Sigma> = BS vs sfs \<and> [c] = ufcs cd vs \<and> [] = ufsfs cd sfs" 
     by (metis unfl_state)
   moreover then obtain v where "vs = [v] \<and> c = unflatten_closure cd v" by blast
   ultimately show ?thesis by simp
 qed
 
-lemma evalb_end [simp]: "iter (\<leadsto>\<^sub>e\<^sub>c\<^sub>o) (unflatten_state cd\<^sub>b \<Sigma>\<^sub>b) (TCOS [c] []) \<Longrightarrow> 
+lemma evalb_end [simp]: "iter (\<leadsto>\<^sub>e) (unflatten_state cd\<^sub>b \<Sigma>\<^sub>b) (S\<^sub>e [c] []) \<Longrightarrow> 
   orderly_state cd\<^sub>b \<Sigma>\<^sub>b \<Longrightarrow> 
     \<exists>v. iter (\<tturnstile> cd\<^sub>b \<leadsto>\<^sub>b) \<Sigma>\<^sub>b (BS [v] []) \<and> c = unflatten_closure cd\<^sub>b v"
 proof -
-  assume "iter (\<leadsto>\<^sub>e\<^sub>c\<^sub>o) (unflatten_state cd\<^sub>b \<Sigma>\<^sub>b) (TCOS [c] [])"
+  assume "iter (\<leadsto>\<^sub>e) (unflatten_state cd\<^sub>b \<Sigma>\<^sub>b) (S\<^sub>e [c] [])"
   moreover assume O: "orderly_state cd\<^sub>b \<Sigma>\<^sub>b"
-  ultimately obtain \<Sigma>\<^sub>b' where E: "iter (\<tturnstile> cd\<^sub>b \<leadsto>\<^sub>b) \<Sigma>\<^sub>b \<Sigma>\<^sub>b' \<and> unflatten_state cd\<^sub>b \<Sigma>\<^sub>b' = TCOS [c] []" 
+  ultimately obtain \<Sigma>\<^sub>b' where E: "iter (\<tturnstile> cd\<^sub>b \<leadsto>\<^sub>b) \<Sigma>\<^sub>b \<Sigma>\<^sub>b' \<and> unflatten_state cd\<^sub>b \<Sigma>\<^sub>b' = S\<^sub>e [c] []" 
     by fastforce
   moreover with O have "orderly_state cd\<^sub>b \<Sigma>\<^sub>b'" by fastforce
   moreover with E obtain v where "\<Sigma>\<^sub>b' = BS [v] [] \<and> c = unflatten_closure cd\<^sub>b v" 
