Printing.thy
@@ -1,7 +1,7 @@
 theory Printing
   imports "02Typed/Typechecking" "03Debruijn/NameRemoval" "05Closure/ClosureConversion" 
-    "06TreeCode/TreeCodeConversion" "07TailCall/TailCallOptimization" "08ByteCode/CodeFlattening" 
-    "09HeapMemory/HeapConversion" "10ChainedEnvironment/Chaining" "11FlatMemory/MemoryFlattening"
+    "06TreeCode/TreeCodeConversion" "06TreeCode/TailCallOptimization" "08ByteCode/CodeFlattening" 
+    "09HeapMemory/HeapConversion" "10ChainedEnvironment/Chaining" "11FlatMemory/MemoryFlattening" 
     "13AssemblyCode/Assemble" "14MachineCode/Disassemble" 
 begin
 
@@ -9,38 +9,34 @@ datatype print = Number nat | Fun
 
 primrec print_nexpr :: "'a expr\<^sub>s \<Rightarrow> print" where
   "print_nexpr (Var\<^sub>s x) = undefined"
-| "print_nexpr (Const\<^sub>s k) = Number k"
+| "print_nexpr (Const\<^sub>s n) = Number n"
 | "print_nexpr (Lam\<^sub>s x t e) = Fun"
 | "print_nexpr (App\<^sub>s e\<^sub>1 e\<^sub>2) = undefined"
 
 primrec print_dexpr :: "expr\<^sub>d \<Rightarrow> print" where
   "print_dexpr (Var\<^sub>d x) = undefined"
-| "print_dexpr (Const\<^sub>d k) = Number k"
+| "print_dexpr (Const\<^sub>d n) = Number n"
 | "print_dexpr (Lam\<^sub>d t e) = Fun"
 | "print_dexpr (App\<^sub>d e\<^sub>1 e\<^sub>2) = undefined"
 
 primrec print_closure :: "closure\<^sub>c \<Rightarrow> print" where
-  "print_closure (Const\<^sub>c k) = Number k"
+  "print_closure (Const\<^sub>c n) = Number n"
 | "print_closure (Lam\<^sub>c t cs e) = Fun"
 
-primrec print_tclosure :: "closure\<^sub>e \<Rightarrow> print" where
-  "print_tclosure (Const\<^sub>e k) = Number k"
-| "print_tclosure (Lam\<^sub>e cs cd) = Fun"
-
-primrec print_tco_closure :: "tco_closure \<Rightarrow> print" where
-  "print_tco_closure (TCOConst k) = Number k"
-| "print_tco_closure (TCOLam cs cd r) = Fun"
+primrec print_eclosure :: "closure\<^sub>e \<Rightarrow> print" where
+  "print_eclosure (Const\<^sub>e n) = Number n"
+| "print_eclosure (Lam\<^sub>e cs cd r) = Fun"
 
 primrec print_bclosure :: "bclosure \<Rightarrow> print" where
-  "print_bclosure (BConst k) = Number k"
+  "print_bclosure (BConst n) = Number n"
 | "print_bclosure (BLam cs pc) = Fun"
 
 primrec print_hclosure :: "hclosure \<Rightarrow> print" where
-  "print_hclosure (HConst k) = Number k"
+  "print_hclosure (HConst n) = Number n"
 | "print_hclosure (HLam cs pc) = Fun"
 
 primrec print_ceclosure :: "ceclosure \<Rightarrow> print" where
-  "print_ceclosure (CEConst k) = Number k"
+  "print_ceclosure (CEConst n) = Number n"
 | "print_ceclosure (CELam cs pc) = Fun"
 
 fun print_uval :: "(nat \<Rightarrow> nat) \<Rightarrow> nat \<Rightarrow> print" where
@@ -68,13 +64,13 @@ proof (induction c)
   thus ?case by (induction cs arbitrary: e) simp_all
 qed simp_all
 
-lemma [simp]: "print_tco_closure (tco_val c) = print_tclosure c"
+lemma [simp]: "print_eclosure (tco_val c) = print_eclosure c"
   by (induction c) simp_all
 
-lemma [simp]: "print_tclosure (encode_closure c) = print_closure c" 
+lemma [simp]: "print_eclosure (encode_closure c) = print_closure c" 
   by (induction c) (simp_all del: print_eqiv_declosure)
 
-lemma [simp]: "print_bclosure c = print_tco_closure (unflatten_closure cd c)" 
+lemma [simp]: "print_bclosure c = print_eclosure (unflatten_closure cd c)" 
   by (induction c) simp_all
 
 lemma [simp]: "print_hclosure (hlookup h x) = print_bclosure (unheap_closure h x)"
