06TreeCode/TailCallOptimization.thy
@@ -1,0 +1,423 @@
+theory TailCallOptimization
+  imports TreeCode "../00Utils/Iteration"
+begin
+
+subsection \<open>Tail-Call Optimization\<close>
+
+text \<open>A tail-call is a function call that takes place at the very end of another function's body. 
+The significance of this becomes clear when you consider the naive execution of such a function. The 
+last thing the outer function does before it returns is to call the inner function; then, when the 
+inner function returns, the outer function immediately returns too. The outer function's stack frame 
+remains in the stack the whole time the inner function is executing, despite the fact that it will 
+never be needed again. Tail-call optimization changes the push into the inner function into a 
+_jump_ to the inner function, replacing the one frame with the other - the call stack is shorter, 
+and execution is quicker too, since the effort of preserving and then popping the outer frame is 
+avoided. When applied systematically the effect can be quite great: notably, recursive functions 
+that only make recursive calls in tail-position ("tail-recursive functions") can be executed in 
+constant space, just like an imperative loop. This is precisely what we added the \<open>Jump\<^sub>e\<close> 
+instruction to express.\<close>
+
+text \<open>What exactly do we change with tail-call optimization? We replace every sequence of an
+\<open>Apply\<^sub>e\<close> followed by a \<open>Return\<^sub>e\<close> with a \<open>Jump\<^sub>e\<close>, obviously. But we also eliminate certain frames from
+the call stack; specifically, any frame that consists of an empty codeblock followed by a \<open>Return\<^sub>e\<close>.
+We mark these frames as \<open>dead_frame\<close>s.\<close>
+
+fun dead_frame :: "frame\<^sub>e \<Rightarrow> bool" where
+  "dead_frame (\<V>, [], Return\<^sub>e) = True"
+| "dead_frame (\<V>, [], Jump\<^sub>e) = False"
+| "dead_frame (\<V>, op # \<C>, r) = False"
+
+text \<open>The optimization itself is simple: we convert the code and returns, then map the conversion up 
+through the levels of the state, taking care to eliminate the dead frames in the stack:\<close>
+
+primrec tco_return :: "code\<^sub>e list \<Rightarrow> return\<^sub>e \<Rightarrow> return\<^sub>e" where
+  "tco_return [] r = r"
+| "tco_return (op # cd) r = (if op = Apply\<^sub>e \<and> cd = [] then Jump\<^sub>e else tco_return cd r)"
+
+fun tco_code :: "code\<^sub>e list \<Rightarrow> code\<^sub>e list" where
+  "tco_code [] = []"
+| "tco_code (Apply\<^sub>e # []) = []"
+| "tco_code (PushLam\<^sub>e \<C>' r # \<C>) = PushLam\<^sub>e (tco_code \<C>') (tco_return \<C>' r) # tco_code \<C>"
+| "tco_code (op # \<C>) = op # tco_code \<C>"
+
+primrec tco_val :: "closure\<^sub>e \<Rightarrow> closure\<^sub>e" where
+  "tco_val (Const\<^sub>e n) = Const\<^sub>e n"
+| "tco_val (Lam\<^sub>e \<Delta> \<C> r) = Lam\<^sub>e (map tco_val \<Delta>) (tco_code \<C>) (tco_return \<C> r)"
+
+fun tco_frame :: "frame\<^sub>e \<Rightarrow> frame\<^sub>e" where
+  "tco_frame (\<Delta>, \<C>, r) = (map tco_val \<Delta>, tco_code \<C>, tco_return \<C> r)"
+
+abbreviation tco_stack :: "frame\<^sub>e list \<Rightarrow> frame\<^sub>e list" where
+  "tco_stack s \<equiv> filter (\<lambda>f. \<not> dead_frame f) (map tco_frame s)"
+
+primrec tco_state :: "state\<^sub>e \<Rightarrow> state\<^sub>e" where
+  "tco_state (S\<^sub>e \<V> s) = S\<^sub>e (map tco_val \<V>) (tco_stack s)"
+
+text \<open>We will of course prove that tail-call removal is semantics-preserving, but we will not 
+formally prove that it really is "an optimization". Instead, we will prove some much simpler results 
+that indicate _why_ it is an optimization, and what a full proof would need to formalize.\<close>
+
+text \<open>The optimized code is always shorter. Since tail-call removal is a local optimization, leaving 
+the global structure of the computation intact, any codeblock executed before it will be executed 
+after as well. Assuming that each operation takes roughly equal time, this means that tail-call 
+optimization reduces runtime. (In fact, we will see much later that \<open>Jump\<^sub>e\<close> is shorter to run as 
+machine code than the \<open>Apply\<^sub>e; Return\<^sub>e\<close> sequence, so we do even better. But we're not there yet.)\<close>
+
+theorem tco_always_shorter_code [simp]: "length (tco_code \<C>) \<le> length \<C>"
+  by (induction \<C> rule: tco_code.induct) simp_all
+
+text \<open>The value stack - what we might consider something like a proxy for the heap usage - is 
+unchanged by tail-call removal. But the call stack - which remains the call stack throughout 
+compilation - is made shorter:\<close>
+
+primrec get_callstack :: "state\<^sub>e \<Rightarrow> frame\<^sub>e list" where
+  "get_callstack (S\<^sub>e \<V> s) = s"
+
+theorem tco_always_smaller_stack [simp]: "
+    length (get_callstack (tco_state \<Sigma>)) \<le> length (get_callstack \<Sigma>)"
+  by (induction \<Sigma>) simp_all
+
+text \<open>Correctness is the easier proof for this pass. First off, we need some auxiliary functions to 
+express that no \<open>PushLam\<^sub>e\<close> contains code for a dead frame, and every return is a \<open>Return\<^sub>e\<close> (as will
+always be the case, pre-optimization).\<close>
+
+fun complete_lams :: "code\<^sub>e list \<Rightarrow> bool" where
+  "complete_lams [] = True"
+| "complete_lams (PushLam\<^sub>e \<C>' r # \<C>) = (\<C>' \<noteq> [] \<and> r = Return\<^sub>e \<and> complete_lams \<C>' \<and> complete_lams \<C>)"
+| "complete_lams (op # \<C>) = complete_lams \<C>"
+
+primrec complete_lams_val :: "closure\<^sub>e \<Rightarrow> bool" where
+  "complete_lams_val (Const\<^sub>e n) = True"
+| "complete_lams_val (Lam\<^sub>e \<Delta> \<C> r) = 
+    (\<C> \<noteq> [] \<and> r = Return\<^sub>e \<and> list_all complete_lams_val \<Delta> \<and> complete_lams \<C>)"
+
+fun complete_lams_frame :: "frame\<^sub>e \<Rightarrow> bool" where
+  "complete_lams_frame (\<Delta>, \<C>, r) = (list_all complete_lams_val \<Delta> \<and> complete_lams \<C> \<and> r = Return\<^sub>e)"
+
+primrec complete_lams_state :: "state\<^sub>e \<Rightarrow> bool" where
+  "complete_lams_state (S\<^sub>e \<V> s) = (list_all complete_lams_val \<V> \<and> list_all complete_lams_frame s)"
+
+lemma eval_complete_lams [simp]: "\<Sigma> \<leadsto>\<^sub>e \<Sigma>' \<Longrightarrow> complete_lams_state \<Sigma> \<Longrightarrow> complete_lams_state \<Sigma>'"
+  by (induction \<Sigma> \<Sigma>' rule: eval\<^sub>e.induct) auto
+
+text \<open>The \<open>iter (\<leadsto>\<^sub>e)\<close> in correctness is unusual, in that it doesn't merely mean one-or-more 
+evaluation steps, or zero-or-one, but either: clearing a dead stack frame incorporates an extra step 
+in every case except \<open>ev\<^sub>e_return\<close>, where the optimization pass has already cleared the dead frame 
+for us and it takes no steps. It may seem odd that the optimized code requires two steps where the 
+original code needed one, but what is actually happening is the "missing" steps from the 
+\<open>ev\<^sub>e_return\<close> are being moved there; we are still reducing the number of steps steps in total.\<close>
+
+lemma tco_to_dead_frame [simp]: "dead_frame (\<Delta>, tco_code \<C>, tco_return \<C> r) = (\<C> = [] \<and> r = Return\<^sub>e)"
+proof (induction \<C> rule: tco_code.induct)
+  case 1
+  thus ?case by (induction r) simp_all
+qed simp_all
+
+lemma tco_to_dead_frame_apply [simp]: "
+  dead_frame (map tco_val \<Delta>, tco_code (Apply\<^sub>e # \<C>), tco_return \<C> r) = (\<C> = [] \<and> r = Return\<^sub>e)"
+proof (induction \<C> rule: tco_code.induct)
+  case 1
+  thus ?case by (induction r) simp_all
+qed simp_all
+
+theorem correctness\<^sub>t\<^sub>c\<^sub>o: "\<Sigma> \<leadsto>\<^sub>e \<Sigma>' \<Longrightarrow> complete_lams_state \<Sigma> \<Longrightarrow> 
+  iter (\<leadsto>\<^sub>e) (tco_state \<Sigma>) (tco_state \<Sigma>')"
+proof (induction \<Sigma> \<Sigma>' rule: eval\<^sub>e.induct)
+  case (ev\<^sub>e_lookup \<Delta> x v \<V> \<C> r s)
+  thus ?case
+  proof (cases "\<C> = []")
+    case True
+    with ev\<^sub>e_lookup have  "
+      S\<^sub>e (tco_val v # map tco_val \<V>) ((map tco_val \<Delta>, tco_code \<C>, tco_return \<C> r) # tco_stack s) \<leadsto>\<^sub>e
+        S\<^sub>e (tco_val v # map tco_val \<V>) (tco_stack s)" by simp
+    moreover from ev\<^sub>e_lookup have "
+      S\<^sub>e (map tco_val \<V>) ((map tco_val \<Delta>, Lookup\<^sub>e x # tco_code \<C>, tco_return \<C> r) # tco_stack s) \<leadsto>\<^sub>e
+        S\<^sub>e (tco_val v # map tco_val \<V>) ((map tco_val \<Delta>, tco_code \<C>, tco_return \<C> r) # tco_stack s)"
+      by simp
+    ultimately have "iter (\<leadsto>\<^sub>e) (S\<^sub>e (map tco_val \<V>) 
+      ((map tco_val \<Delta>, Lookup\<^sub>e x # tco_code \<C>, tco_return \<C> r) # tco_stack s))
+        (S\<^sub>e (tco_val v # map tco_val \<V>) (tco_stack s))"
+      by (metis (no_types, lifting) iter_refl iter_step)
+    with ev\<^sub>e_lookup True show ?thesis by simp
+  next
+    case False
+    with ev\<^sub>e_lookup have "tco_state (S\<^sub>e \<V> ((\<Delta>, Lookup\<^sub>e x # \<C>, r) # s)) \<leadsto>\<^sub>e
+      tco_state (S\<^sub>e (v # \<V>) ((\<Delta>, \<C>, r) # s))" by auto
+    thus ?thesis by (metis iter_one)
+  qed
+next
+  case (ev\<^sub>e_pushcon \<V> \<Delta> n \<C> r s)
+  thus ?case
+  proof (cases "\<C> = []")
+    case True
+    with ev\<^sub>e_pushcon have "
+      S\<^sub>e (Const\<^sub>e n # map tco_val \<V>) ((map tco_val \<Delta>, tco_code \<C>, tco_return \<C> r) # tco_stack s) \<leadsto>\<^sub>e 
+        S\<^sub>e (Const\<^sub>e n # map tco_val \<V>) (tco_stack s)" by simp
+    moreover have "
+      S\<^sub>e (map tco_val \<V>) ((map tco_val \<Delta>, PushCon\<^sub>e n # tco_code \<C>, tco_return \<C> r) # tco_stack s) \<leadsto>\<^sub>e 
+        S\<^sub>e (Const\<^sub>e n # map tco_val \<V>) ((map tco_val \<Delta>, tco_code \<C>, tco_return \<C> r) # tco_stack s)"
+      by simp
+    ultimately have "iter (\<leadsto>\<^sub>e) (S\<^sub>e (map tco_val \<V>) 
+      ((map tco_val \<Delta>, PushCon\<^sub>e n # tco_code \<C>, tco_return \<C> r) # tco_stack s))
+        (S\<^sub>e (Const\<^sub>e n # map tco_val \<V>) (tco_stack s))"
+      by (metis (no_types, lifting) iter_refl iter_step)
+    with ev\<^sub>e_pushcon True show ?thesis by simp
+  next
+    case False
+    hence "tco_state (S\<^sub>e \<V> ((\<Delta>, PushCon\<^sub>e n # \<C>, r) # s)) \<leadsto>\<^sub>e 
+      tco_state (S\<^sub>e (Const\<^sub>e n # \<V>) ((\<Delta>, \<C>, r) # s))" by auto
+    thus ?thesis by (metis iter_one)
+  qed
+next
+  case (ev\<^sub>e_pushlam \<V> \<Delta> \<C>' r' \<C> r s)
+  thus ?case
+  proof (cases "\<C> = []")
+    case True
+    with ev\<^sub>e_pushlam have "S\<^sub>e (Lam\<^sub>e (map tco_val \<Delta>) (tco_code \<C>') (tco_return \<C>' r') # map tco_val \<V>) 
+      ((map tco_val \<Delta>, tco_code \<C>, tco_return \<C> r) # tco_stack s) \<leadsto>\<^sub>e 
+      S\<^sub>e (Lam\<^sub>e (map tco_val \<Delta>) (tco_code \<C>') (tco_return \<C>' r') # map tco_val \<V>) (tco_stack s)" 
+        by simp
+    moreover have "S\<^sub>e (map tco_val \<V>) ((map tco_val \<Delta>, PushLam\<^sub>e (tco_code \<C>') (tco_return \<C>' r') # 
+      tco_code \<C>, tco_return \<C> r) # tco_stack s) \<leadsto>\<^sub>e 
+      S\<^sub>e (Lam\<^sub>e (map tco_val \<Delta>) (tco_code \<C>') (tco_return \<C>' r') # map tco_val \<V>) 
+      ((map tco_val \<Delta>, tco_code \<C>, tco_return \<C> r) # tco_stack s)"
+        by simp
+    ultimately have "iter (\<leadsto>\<^sub>e) (S\<^sub>e (map tco_val \<V>) ((map tco_val \<Delta>, PushLam\<^sub>e (tco_code \<C>') 
+      (tco_return \<C>' r') # tco_code \<C>, tco_return \<C> r) # tco_stack s))
+      (S\<^sub>e (Lam\<^sub>e (map tco_val \<Delta>) (tco_code \<C>') (tco_return \<C>' r') # map tco_val \<V>) (tco_stack s))"
+      by (metis (no_types, lifting) iter_refl iter_step)
+    with ev\<^sub>e_pushlam True show ?thesis by simp
+  next
+    case False
+    hence "tco_state (S\<^sub>e \<V> ((\<Delta>, PushLam\<^sub>e \<C>' r' # \<C>, r) # s)) \<leadsto>\<^sub>e 
+      tco_state (S\<^sub>e (Lam\<^sub>e \<Delta> \<C>' r' # \<V>) ((\<Delta>, \<C>, r) # s))" by simp
+    thus ?thesis by (metis iter_one)
+  qed
+next
+  case (ev\<^sub>e_apply v \<Delta>' \<C>' r' \<V> \<Delta> \<C> r s)
+  thus ?case
+  proof (cases "\<C> = []")
+    case True
+    with ev\<^sub>e_apply have "tco_state (S\<^sub>e (v # Lam\<^sub>e \<Delta>' \<C>' r' # \<V>) ((\<Delta>, Apply\<^sub>e # \<C>, r) # s)) \<leadsto>\<^sub>e
+      tco_state (S\<^sub>e \<V> ((v # \<Delta>', \<C>', r') # (\<Delta>, \<C>, r) # s))" by auto
+    thus ?thesis by (metis iter_one)
+  next
+    case False
+    with ev\<^sub>e_apply have "tco_state (S\<^sub>e (v # Lam\<^sub>e \<Delta>' \<C>' r' # \<V>) ((\<Delta>, Apply\<^sub>e # \<C>, r) # s)) \<leadsto>\<^sub>e 
+      tco_state (S\<^sub>e \<V> ((v # \<Delta>', \<C>', r') # (\<Delta>, \<C>, r) # s))" 
+      by (cases \<C> rule: tco_code.cases) simp_all
+    thus ?thesis by (metis iter_one)
+  qed
+qed simp_all
+
+lemma correctness\<^sub>t\<^sub>c\<^sub>o_iter: "iter (\<leadsto>\<^sub>e) \<Sigma> \<Sigma>' \<Longrightarrow> complete_lams_state \<Sigma> \<Longrightarrow> 
+  iter (\<leadsto>\<^sub>e) (tco_state \<Sigma>) (tco_state \<Sigma>')"
+proof (induction \<Sigma> \<Sigma>' rule: iter.induct)
+  case (iter_step \<Sigma> \<Sigma>' \<Sigma>'')
+  hence "iter (\<leadsto>\<^sub>e) (tco_state \<Sigma>') (tco_state \<Sigma>'')" by simp
+  moreover from iter_step have "iter (\<leadsto>\<^sub>e) (tco_state \<Sigma>) (tco_state \<Sigma>')" by (metis correctness\<^sub>t\<^sub>c\<^sub>o)
+  ultimately show ?case by (metis iter_append)
+qed simp_all
+
+text \<open>We now prove the reconstruction lemmas for completeness:\<close>
+
+lemma [dest]: "(\<Delta>\<^sub>t\<^sub>c\<^sub>o, \<C>\<^sub>t\<^sub>c\<^sub>o, r\<^sub>t\<^sub>c\<^sub>o) = tco_frame f\<^sub>e \<Longrightarrow> \<exists>\<Delta>\<^sub>e \<C>\<^sub>e r\<^sub>e. f\<^sub>e = (\<Delta>\<^sub>e, \<C>\<^sub>e, r\<^sub>e) \<and> 
+    \<Delta>\<^sub>t\<^sub>c\<^sub>o = map tco_val \<Delta>\<^sub>e \<and> \<C>\<^sub>t\<^sub>c\<^sub>o = tco_code \<C>\<^sub>e \<and> r\<^sub>t\<^sub>c\<^sub>o = tco_return \<C>\<^sub>e r\<^sub>e"
+  by (induction f\<^sub>e) simp_all
+
+lemma [dest]: "f\<^sub>t\<^sub>c\<^sub>o # s\<^sub>t\<^sub>c\<^sub>o = tco_stack s\<^sub>e \<Longrightarrow> \<exists>s\<^sub>e\<^sub>1 s\<^sub>e\<^sub>2 f\<^sub>e. s\<^sub>e = s\<^sub>e\<^sub>1 @ f\<^sub>e # s\<^sub>e\<^sub>2 \<and> 
+  list_all dead_frame (map tco_frame s\<^sub>e\<^sub>1) \<and> f\<^sub>t\<^sub>c\<^sub>o = tco_frame f\<^sub>e \<and> s\<^sub>t\<^sub>c\<^sub>o = tco_stack s\<^sub>e\<^sub>2"
+proof (induction s\<^sub>e)
+  case (Cons f\<^sub>e s\<^sub>e)
+  thus ?case
+  proof (cases "dead_frame (tco_frame f\<^sub>e)")
+    case True
+    with Cons obtain s\<^sub>e\<^sub>1 s\<^sub>e\<^sub>2 f\<^sub>e' where "s\<^sub>e = s\<^sub>e\<^sub>1 @ f\<^sub>e' # s\<^sub>e\<^sub>2 \<and> list_all dead_frame (map tco_frame s\<^sub>e\<^sub>1) \<and> 
+      f\<^sub>t\<^sub>c\<^sub>o = tco_frame f\<^sub>e' \<and> s\<^sub>t\<^sub>c\<^sub>o = tco_stack s\<^sub>e\<^sub>2" by auto
+    with True have "f\<^sub>e # s\<^sub>e = (f\<^sub>e # s\<^sub>e\<^sub>1) @ f\<^sub>e' # s\<^sub>e\<^sub>2 \<and> list_all dead_frame (map tco_frame (f\<^sub>e # s\<^sub>e\<^sub>1)) \<and> 
+      f\<^sub>t\<^sub>c\<^sub>o = tco_frame f\<^sub>e' \<and> s\<^sub>t\<^sub>c\<^sub>o = tco_stack s\<^sub>e\<^sub>2" by simp
+    thus ?thesis by blast
+  next
+    case False
+    with Cons have "f\<^sub>e # s\<^sub>e = [] @ f\<^sub>e # s\<^sub>e \<and> list_all dead_frame (map tco_frame []) \<and> 
+      f\<^sub>t\<^sub>c\<^sub>o = tco_frame f\<^sub>e \<and> s\<^sub>t\<^sub>c\<^sub>o = tco_stack s\<^sub>e" by simp
+    thus ?thesis by blast
+  qed
+qed simp_all
+
+lemma [dest]: "S\<^sub>e \<V>\<^sub>t\<^sub>c\<^sub>o s\<^sub>t\<^sub>c\<^sub>o = tco_state \<Sigma>\<^sub>e \<Longrightarrow> 
+    \<exists>\<V>\<^sub>e s\<^sub>e. \<Sigma>\<^sub>e = S\<^sub>e \<V>\<^sub>e s\<^sub>e \<and> \<V>\<^sub>t\<^sub>c\<^sub>o = map tco_val \<V>\<^sub>e \<and> s\<^sub>t\<^sub>c\<^sub>o = tco_stack s\<^sub>e"
+  by (induction \<Sigma>\<^sub>e) simp_all
+
+text \<open>Completeness then follows:\<close>
+
+theorem complete\<^sub>t\<^sub>c\<^sub>o [simp]: "tco_state \<Sigma>\<^sub>e \<leadsto>\<^sub>e \<Sigma>\<^sub>t\<^sub>c\<^sub>o' \<Longrightarrow> 
+  \<exists>\<Sigma>\<^sub>e'. iter (\<leadsto>\<^sub>e) \<Sigma>\<^sub>e \<Sigma>\<^sub>e' \<and> \<Sigma>\<^sub>t\<^sub>c\<^sub>o' = tco_state \<Sigma>\<^sub>e'"
+proof (induction "tco_state \<Sigma>\<^sub>e" \<Sigma>\<^sub>t\<^sub>c\<^sub>o' rule: eval\<^sub>e.induct)
+  case (ev\<^sub>e_lookup \<Delta>\<^sub>t\<^sub>c\<^sub>o x v \<V>\<^sub>t\<^sub>c\<^sub>o \<C>\<^sub>t\<^sub>c\<^sub>o r\<^sub>t\<^sub>c\<^sub>o s\<^sub>t\<^sub>c\<^sub>o)
+  then obtain \<V>\<^sub>e s\<^sub>e\<^sub>1 s\<^sub>e\<^sub>2 \<Delta>\<^sub>e \<C>\<^sub>e r\<^sub>e where "\<Sigma>\<^sub>e = S\<^sub>e \<V>\<^sub>e (s\<^sub>e\<^sub>1 @ (\<Delta>\<^sub>e, \<C>\<^sub>e, r\<^sub>e) # s\<^sub>e\<^sub>2) \<and> \<V>\<^sub>t\<^sub>c\<^sub>o = map tco_val \<V>\<^sub>e \<and> 
+    list_all dead_frame (map tco_frame s\<^sub>e\<^sub>1) \<and> \<Delta>\<^sub>t\<^sub>c\<^sub>o = map tco_val \<Delta>\<^sub>e \<and> Lookup\<^sub>e x # \<C>\<^sub>t\<^sub>c\<^sub>o = tco_code \<C>\<^sub>e \<and> 
+      r\<^sub>t\<^sub>c\<^sub>o = tco_return \<C>\<^sub>e r\<^sub>e \<and> s\<^sub>t\<^sub>c\<^sub>o = tco_stack s\<^sub>e\<^sub>2" by fast
+
+
+
+  have "iter (\<leadsto>\<^sub>e) \<Sigma>\<^sub>e \<Sigma>\<^sub>e' \<and> S\<^sub>e (v # \<V>\<^sub>t\<^sub>c\<^sub>o) ((\<Delta>\<^sub>t\<^sub>c\<^sub>o, \<C>\<^sub>t\<^sub>c\<^sub>o, r\<^sub>t\<^sub>c\<^sub>o) # s\<^sub>t\<^sub>c\<^sub>o) = tco_state \<Sigma>\<^sub>e'" by simp
+  thus ?case by blast
+next
+  case (ev\<^sub>e_pushcon \<V>\<^sub>t\<^sub>c\<^sub>o \<Delta>\<^sub>t\<^sub>c\<^sub>o n \<C>\<^sub>t\<^sub>c\<^sub>o r\<^sub>t\<^sub>c\<^sub>o s\<^sub>t\<^sub>c\<^sub>o)
+  then obtain \<V>\<^sub>e s\<^sub>e\<^sub>1 s\<^sub>e\<^sub>2 f\<^sub>e where "\<Sigma>\<^sub>e = S\<^sub>e \<V>\<^sub>e (s\<^sub>e\<^sub>1 @ f\<^sub>e # s\<^sub>e\<^sub>2) \<and> \<V>\<^sub>t\<^sub>c\<^sub>o = map tco_val \<V>\<^sub>e \<and> 
+    list_all dead_frame (map tco_frame s\<^sub>e\<^sub>1) \<and> (\<Delta>\<^sub>t\<^sub>c\<^sub>o, PushCon\<^sub>e n # \<C>\<^sub>t\<^sub>c\<^sub>o, r\<^sub>t\<^sub>c\<^sub>o) = tco_frame f\<^sub>e \<and> 
+      s\<^sub>t\<^sub>c\<^sub>o = tco_stack s\<^sub>e\<^sub>2" by blast
+
+  then show ?case by simp
+next
+  case (ev\<^sub>e_pushlam \<V>\<^sub>t\<^sub>c\<^sub>o \<Delta>\<^sub>t\<^sub>c\<^sub>o \<C>' r' \<C>\<^sub>t\<^sub>c\<^sub>o r\<^sub>t\<^sub>c\<^sub>o s\<^sub>t\<^sub>c\<^sub>o)
+  then obtain \<V>\<^sub>e s\<^sub>e\<^sub>1 s\<^sub>e\<^sub>2 f\<^sub>e where "\<Sigma>\<^sub>e = S\<^sub>e \<V>\<^sub>e (s\<^sub>e\<^sub>1 @ f\<^sub>e # s\<^sub>e\<^sub>2) \<and> \<V>\<^sub>t\<^sub>c\<^sub>o = map tco_val \<V>\<^sub>e \<and> 
+    list_all dead_frame (map tco_frame s\<^sub>e\<^sub>1) \<and> (\<Delta>\<^sub>t\<^sub>c\<^sub>o, PushLam\<^sub>e \<C>' r' # \<C>\<^sub>t\<^sub>c\<^sub>o, r\<^sub>t\<^sub>c\<^sub>o) = tco_frame f\<^sub>e \<and> 
+      s\<^sub>t\<^sub>c\<^sub>o = tco_stack s\<^sub>e\<^sub>2" by blast
+
+  then show ?case by simp
+next
+  case (ev\<^sub>e_apply v \<Delta>' \<C>' r' \<V>\<^sub>t\<^sub>c\<^sub>o \<Delta>\<^sub>t\<^sub>c\<^sub>o \<C>\<^sub>t\<^sub>c\<^sub>o r\<^sub>t\<^sub>c\<^sub>o s\<^sub>t\<^sub>c\<^sub>o)
+  then obtain \<V>\<^sub>e s\<^sub>e\<^sub>1 s\<^sub>e\<^sub>2 f\<^sub>e where "\<Sigma>\<^sub>e = S\<^sub>e \<V>\<^sub>e (s\<^sub>e\<^sub>1 @ f\<^sub>e # s\<^sub>e\<^sub>2) \<and> (v # Lam\<^sub>e \<Delta>' \<C>' r' # \<V>\<^sub>t\<^sub>c\<^sub>o) = map tco_val \<V>\<^sub>e \<and> 
+    list_all dead_frame (map tco_frame s\<^sub>e\<^sub>1) \<and> (\<Delta>\<^sub>t\<^sub>c\<^sub>o, Apply\<^sub>e # \<C>\<^sub>t\<^sub>c\<^sub>o, r\<^sub>t\<^sub>c\<^sub>o) = tco_frame f\<^sub>e \<and> 
+      s\<^sub>t\<^sub>c\<^sub>o = tco_stack s\<^sub>e\<^sub>2" by blast
+
+  then show ?case by simp
+next
+  case (ev\<^sub>e_return \<V>\<^sub>t\<^sub>c\<^sub>o \<Delta>\<^sub>t\<^sub>c\<^sub>o s\<^sub>t\<^sub>c\<^sub>o)
+  then obtain \<V>\<^sub>e s\<^sub>e\<^sub>1 s\<^sub>e\<^sub>2 f\<^sub>e where "\<Sigma>\<^sub>e = S\<^sub>e \<V>\<^sub>e (s\<^sub>e\<^sub>1 @ f\<^sub>e # s\<^sub>e\<^sub>2) \<and> \<V>\<^sub>t\<^sub>c\<^sub>o = map tco_val \<V>\<^sub>e \<and> 
+    list_all dead_frame (map tco_frame s\<^sub>e\<^sub>1) \<and> (\<Delta>\<^sub>t\<^sub>c\<^sub>o, [], Return\<^sub>e) = tco_frame f\<^sub>e \<and> 
+      s\<^sub>t\<^sub>c\<^sub>o = tco_stack s\<^sub>e\<^sub>2" by blast
+
+  then show ?case by simp
+next
+  case (ev\<^sub>e_jump v \<Delta>' \<C>' r' \<V>\<^sub>t\<^sub>c\<^sub>o \<Delta>\<^sub>t\<^sub>c\<^sub>o s\<^sub>t\<^sub>c\<^sub>o)
+  then obtain \<V>\<^sub>e s\<^sub>e\<^sub>1 s\<^sub>e\<^sub>2 f\<^sub>e where "\<Sigma>\<^sub>e = S\<^sub>e \<V>\<^sub>e (s\<^sub>e\<^sub>1 @ f\<^sub>e # s\<^sub>e\<^sub>2) \<and> (v # Lam\<^sub>e \<Delta>' \<C>' r' # \<V>\<^sub>t\<^sub>c\<^sub>o) = map tco_val \<V>\<^sub>e \<and> 
+    list_all dead_frame (map tco_frame s\<^sub>e\<^sub>1) \<and> (\<Delta>\<^sub>t\<^sub>c\<^sub>o, [], Jump\<^sub>e) = tco_frame f\<^sub>e \<and> 
+      s\<^sub>t\<^sub>c\<^sub>o = tco_stack s\<^sub>e\<^sub>2" by blast
+
+  then show ?case by simp
+qed
+
+(*
+lemma [simp]: "cd \<noteq> [] \<Longrightarrow> tco_r (op # cd) = tco_r cd"
+  by (induction op) (simp_all split: list.splits)
+
+lemma tco_r_append [simp]: "cd' \<noteq> [] \<Longrightarrow> tco_r (cd @ cd') = tco_r cd'"
+  by (induction cd) simp_all
+
+lemma [simp]: "cd \<noteq> [] \<Longrightarrow> cd' \<noteq> [] \<Longrightarrow> tco_cd (cd @ cd') \<noteq> []"
+  by (induction cd rule: tco_cd.induct) (simp_all split: list.splits)
+
+lemma [dest]: "(env, cd, r) # sfs = tco_stack sfs' \<Longrightarrow> \<exists>dsfs env' cd' sfs''. 
+  sfs' = dsfs @ (env', cd') # sfs'' \<and> env = map tco_val env' \<and> cd = tco_cd cd' \<and> 
+    r = tco_r cd' \<and> list_all dead_frame dsfs \<and> sfs = tco_stack sfs''"
+proof (induction sfs')
+  case (Cons sf sfs')
+  thus ?case
+  proof (induction sf)
+    case (Pair env' cd')
+    thus ?case
+    proof (induction cd' rule: tco_cd.induct)
+      case 1
+      then obtain dsfs env'' cd' sfs'' where X: "sfs' = dsfs @ (env'', cd') # sfs'' \<and> 
+        env = map tco_val env'' \<and> cd = tco_cd cd' \<and> r = tco_r cd' \<and> list_all dead_frame dsfs \<and> 
+          sfs = tco_stack sfs''" by auto
+      hence "\<exists>dsfsx. (env', []) # dsfs @ (env'', cd') # sfs'' = dsfsx @ (env'', cd') # sfs'' \<and> 
+          list_all dead_frame dsfsx \<and> sfs = tco_stack sfs''" by simp
+      hence "\<exists>dsfsx sfs'''. 
+        (env', []) # dsfs @ (env'', cd') # sfs'' = dsfsx @ (env'', cd') # sfs''' \<and> 
+          list_all dead_frame dsfsx \<and> sfs = tco_stack sfs'''" by fastforce
+      with X show ?case by fastforce
+    next
+      case (2 x cd')
+      hence "env = map tco_val env' \<and> cd = Lookup\<^sub>e x # tco_cd cd' \<and> r = tco_r cd' \<and> 
+        sfs = tco_stack sfs'" by simp
+      thus ?case by fastforce
+    next
+      case (3 k cd')
+      hence "env = map tco_val env' \<and> cd = PushCon\<^sub>e k # tco_cd cd' \<and> r = tco_r cd' \<and> 
+        sfs = tco_stack sfs'" by simp
+      thus ?case by fastforce
+    next
+      case (4 cd\<^sub>e cd')
+      hence "env = map tco_val env' \<and> cd = PushLam\<^sub>e (tco_cd cd\<^sub>e) (tco_r cd\<^sub>e) # tco_cd cd' \<and> 
+        r = tco_r cd' \<and> sfs = tco_stack sfs'" by simp
+      thus ?case by fastforce
+    next
+      case (5 cd')
+      thus ?case
+      proof (cases cd')
+        case Nil
+        moreover with 5 have "env = map tco_val env' \<and> cd = [] \<and> r = Jump\<^sub>e \<and> sfs = tco_stack sfs'" 
+          by simp
+        ultimately show ?thesis by fastforce
+      next
+        case (Cons op cd'')
+        moreover with 5 have "env = map tco_val env' \<and> cd = Apply\<^sub>e # tco_cd (op # cd'') \<and> 
+          r = tco_r (op # cd'') \<and> sfs = tco_stack sfs'" by simp
+        ultimately show ?thesis by fastforce
+      qed
+    qed
+  qed
+qed simp_all
+
+lemma [dest]: "S\<^sub>e vs ((env, cd, r) # sfs) = tco_state \<Sigma> \<Longrightarrow> \<exists>dsfs vs' env' cd' sfs'. 
+  \<Sigma> = S\<^sub>e vs' (dsfs @ (env', cd') # sfs') \<and> vs = map tco_val vs' \<and> env = map tco_val env' \<and> 
+    cd = tco_cd cd' \<and> r = tco_r cd' \<and> list_all dead_frame dsfs \<and> sfs = tco_stack sfs'"
+  by (induction \<Sigma>) auto
+
+lemma [dest]: "Lookup\<^sub>e x # cd = tco_cd cd' \<Longrightarrow> \<exists>cd''. cd' = Lookup\<^sub>e x # cd'' \<and> cd = tco_cd cd''"
+  by (induction cd' rule: tco_cd.induct) (simp_all split: list.splits)
+
+lemma [dest]: "PushCon\<^sub>e k # cd = tco_cd cd' \<Longrightarrow> \<exists>cd''. cd' = PushCon\<^sub>e k # cd'' \<and> cd = tco_cd cd''"
+  by (induction cd' rule: tco_cd.induct) (simp_all split: list.splits)
+
+lemma [dest]: "PushLam\<^sub>e cd' r # cd = tco_cd cd\<^sub>t \<Longrightarrow> \<exists>cd\<^sub>t' cd\<^sub>t''. cd\<^sub>t = PushLam\<^sub>e cd\<^sub>t'' # cd\<^sub>t' \<and> 
+    cd = tco_cd cd\<^sub>t' \<and> r = tco_r cd\<^sub>t'' \<and> cd' = tco_cd cd\<^sub>t''"
+  by (induction cd\<^sub>t rule: tco_cd.induct) (simp_all split: list.splits)
+
+lemma [dest]: "Apply\<^sub>e # cd = tco_cd cd' \<Longrightarrow> 
+    \<exists>op cd''. cd' = Apply\<^sub>e # op # cd'' \<and> cd = tco_cd (op # cd'')"
+  by (induction cd' rule: tco_cd.induct) (simp_all split: list.splits)
+
+lemma [dest]: "Const\<^sub>e k = tco_val v \<Longrightarrow> v = Const\<^sub>e k"
+  by (induction v) simp_all
+
+lemma [dest]: "Lam\<^sub>e env cd r = tco_val v \<Longrightarrow> 
+    \<exists>env\<^sub>t cd\<^sub>t. v = Lam\<^sub>e env\<^sub>t cd\<^sub>t \<and> env = map tco_val env\<^sub>t \<and> cd = tco_cd cd\<^sub>t \<and> r = tco_r cd\<^sub>t"
+  by (induction v) simp_all
+
+lemma [dest]: "Return\<^sub>e = tco_r cd \<Longrightarrow> [] = tco_cd cd \<Longrightarrow> cd = []"
+  by (induction cd rule: tco_cd.induct) (simp_all split: list.splits)
+
+lemma [dest]: "Jump\<^sub>e = tco_r cd \<Longrightarrow> [] = tco_cd cd \<Longrightarrow> cd = [Apply\<^sub>e]"
+  by (induction cd rule: tco_cd.induct) (simp_all split: list.splits)
+
+lemma [simp]: "list_all dead_frame dsfs \<Longrightarrow> iter (\<leadsto>\<^sub>e) (S\<^sub>e vs (dsfs @ sfs)) (S\<^sub>e vs sfs)"
+proof (induction dsfs)
+  case (Cons sf dsfs)
+  then obtain vs' where "sf = (vs', [])" by (cases sf) simp_all
+  hence "S\<^sub>e vs ((sf # dsfs) @ sfs) \<leadsto>\<^sub>e S\<^sub>e vs (dsfs @ sfs)" by simp
+  with Cons show ?case by simp
+qed simp_all
+
+lemma [simp]: "\<not> live_frame fr \<Longrightarrow> iter (\<leadsto>\<^sub>e) (S\<^sub>e vs (fr # sfs)) (S\<^sub>e vs sfs)"
+proof (induction fr rule: live_frame.induct)
+  case (1 env)
+  hence "S\<^sub>e vs ((env, [], Return\<^sub>e) # sfs) \<leadsto>\<^sub>e S\<^sub>e vs sfs" by simp
+  thus ?case by (metis iter_one)
+qed simp_all
+
+lemma [simp]: "tco_cd (op # cd) = [] \<Longrightarrow> tco_r (op # cd) = Jump\<^sub>e"
+  by (induction op) (simp_all split: list.splits)
+
+lemma [simp]: "live_frame (env, cd, Jump\<^sub>e)"
+  by (induction cd) simp_all
+
+lemma tco_never_dead [simp]: "live_frame (env, tco_cd (op # cd), tco_r (op # cd))"
+  by (induction op) (simp_all split: list.splits)
+*)
+
+end
